Feat: Avoid maybe placebos when initialization status is known

Source/DafnyCore/Backends/Rust/Dafny-compiler-rust-definitions.dfy
@@ -148,14 +148,15 @@ module {:extern "Defs"} DafnyToRustCompilerDefinitions {
   // fn Test(i: &mut T) is map["i" := R.BorrowedMut(...)]
   datatype Environment = Environment(
     names: seq<string>,                 // All variable names, after escape, in Rust
-    types: map<string, R.Type>
+    types: map<string, R.Type>,
+    assignmentStatusKnown: set<string> // Variables that are guaranteed to be assigned exactly once
   ) {
     function ToOwned(): Environment {
       this.(types :=
       map k <- types :: k := types[k].ToOwned())
     }
     static function Empty(): Environment {
-      Environment([], map[])
+      Environment([], map[], {})
     }
     opaque predicate CanReadWithoutClone(name: string) {
       name in types && types[name].CanReadWithoutClone()
@@ -181,23 +182,36 @@ module {:extern "Defs"} DafnyToRustCompilerDefinitions {
     function AddAssigned(name: string, tpe: R.Type): Environment
       // If we know for sure the type of name extends the Copy trait
     {
-      Environment(names + [name], types[name := tpe])
+      Environment(names + [name], types[name := tpe], assignmentStatusKnown - {name})
     }
     function merge(other: Environment): Environment
     {
       Environment(
         names + other.names,
-        types + other.types
+        types + other.types,
+        assignmentStatusKnown + other.assignmentStatusKnown
       )
     }
+    // Used to removed from the environment the "_is_assigned" vars used to initialize fields
     function RemoveAssigned(name: string): Environment
       requires name in names
     {
       var indexInEnv := Std.Collections.Seq.IndexOf(names, name);
       Environment(
         names[0..indexInEnv] + names[indexInEnv + 1..],
-        types - {name}
+        types - {name},
+        assignmentStatusKnown - {name}
       )
+    }
+    function AddAssignmentStatusKnown(name: string): Environment {
+      Environment(
+        names,
+        types,
+        assignmentStatusKnown + {name}
+      )
+    }
+    predicate IsAssignmentStatusKnown(name: string) {
+      name in assignmentStatusKnown
     }
   }
 
@@ -701,5 +715,51 @@ module {:extern "Defs"} DafnyToRustCompilerDefinitions {
                                                                                         ]))
             ))
         ]))
+  }
+
+  // Overapproximate but sound static analysis domain for assignment of a variable
+  datatype AssignmentStatus = NotAssigned | SurelyAssigned | Unknown {
+    // After a if, typically. What we know if either of the assignment status is taken
+    function Join(other: AssignmentStatus): AssignmentStatus {
+      if SurelyAssigned? && other.SurelyAssigned? then SurelyAssigned
+      else if NotAssigned? && other.NotAssigned? then NotAssigned
+      else Unknown
+    }
+    function Then(other: AssignmentStatus): AssignmentStatus {
+      if SurelyAssigned? then SurelyAssigned
+      else if NotAssigned? then other
+      else Unknown // It's not as simple. If there are are two paths leading to one being assigned, the other not,
+      // Rust won't be albe to figure out the rules
+    }
+  }
+
+  // What could be problematic is the presence of branches in the assignment
+  // and one branch where a value is not assigned at all.
+  // If return false, we don't know if it's assigned or not
+  function DetectAssignmentStatus(stmts_remainder: seq<Statement>, dafny_name: VarName): AssignmentStatus {
+    if |stmts_remainder| == 0 then NotAssigned else
+    var stmt := stmts_remainder[0];
+    match stmt {
+      case Assign(Ident(assign_name), _) =>
+        if assign_name == dafny_name then SurelyAssigned else
+        DetectAssignmentStatus(stmts_remainder[1..], dafny_name)
+      case If(cond, thn, els) =>
+        DetectAssignmentStatus(thn, dafny_name).Join(DetectAssignmentStatus(els, dafny_name))
+      case Call(on, callName, typeArgs, args, outs) =>
+        if outs.Some? && dafny_name in outs.value then
+          SurelyAssigned
+        else
+          DetectAssignmentStatus(stmts_remainder[1..], dafny_name)
+      case Labeled(_, stmts) =>
+        DetectAssignmentStatus(stmts, dafny_name).Then(DetectAssignmentStatus(stmts_remainder[1..], dafny_name))
+      case DeclareVar(name, _, _) =>
+        if name == dafny_name then
+          NotAssigned // Shadowed
+        else
+          DetectAssignmentStatus(stmts_remainder[1..], dafny_name)
+      case Return(_) | EarlyReturn() | JumpTailCallStart() => NotAssigned
+      case Print(_) => DetectAssignmentStatus(stmts_remainder[1..], dafny_name)
+      case _ => Unknown
+    }
   }
 }
