Source/DafnyCore/Backends/Rust/Dafny-compiler-rust.dfy
@@ -1717,13 +1717,13 @@ module {:extern "DCOMP"} DafnyToRustCompiler {
           }
           case None => {}
         }
-        env := Environment(preAssignNames + paramNames, preAssignTypes + paramTypes);
+        env := Environment(preAssignNames + paramNames, preAssignTypes + paramTypes, {});
 
         var body, _, _ := GenStmts(m.body, selfIdent, env, true, earlyReturn);
 
         fBody := Some(preBody.Then(body));
       } else {
-        env := Environment(paramNames, paramTypes);
+        env := Environment(paramNames, paramTypes, {});
         fBody := None;
       }
       s := R.FnDecl(
@@ -1753,18 +1753,12 @@ module {:extern "DCOMP"} DafnyToRustCompiler {
       var stmts := stmts; // Make it mutable
       while i < |stmts| {
         var stmt := stmts[i];
-        // Avoid lazy initialization if it is not necessary
+        // Avoid maybe placebo wrapping if not necessary
         match stmt {
           case DeclareVar(name, optType, None) =>
-            if i + 1 < |stmts| {
-              match stmts[i + 1] {
-                case Assign(Ident(name2), rhs) =>
-                  if name2 == name {
-                    stmts := stmts[0..i] + [DeclareVar(name, optType, Some(rhs))] + stmts[i+2..];
-                    stmt := stmts[i];
-                  }
-                case _ =>
-              }
+            var laterAssignmentStatus := DetectAssignmentStatus(stmts[i + 1..], name);
+            if !laterAssignmentStatus.Unknown? {
+              newEnv := newEnv.AddAssignmentStatusKnown(escapeVar(name));
             }
           case _ =>
 
@@ -1998,9 +1992,17 @@ module {:extern "DCOMP"} DafnyToRustCompiler {
           }
         }
         case DeclareVar(name, typ, None) => {
-          var newStmt := DeclareVar(name, typ, Some(InitializationValue(typ)));
-          assume {:axiom} newStmt < stmt;
-          generated, readIdents, newEnv := GenStmt(newStmt, selfIdent, env, isLast, earlyReturn);
+          var varName := escapeVar(name);
+          if env.IsAssignmentStatusKnown(varName) {
+            var tpe := GenType(typ, GenTypeContext.default());
+            generated := R.DeclareVar(R.MUT, varName, None, None);
+            readIdents := {};
+            newEnv := env.AddAssigned(varName, tpe);
+          } else {
+            var newStmt := DeclareVar(name, typ, Some(InitializationValue(typ)));
+            assume {:axiom} newStmt < stmt;
+            generated, readIdents, newEnv := GenStmt(newStmt, selfIdent, env, isLast, earlyReturn);
+          }
         }
         case Assign(lhs, expression) => {
           var exprGen, _, exprIdents := GenExpr(expression, selfIdent, env, OwnershipOwned);
@@ -3773,7 +3775,7 @@ module {:extern "DCOMP"} DafnyToRustCompiler {
             paramNames := paramNames + [name];
             paramTypesMap := paramTypesMap[name := params[i].tpe];
           }
-          var subEnv := env.ToOwned().merge(Environment(paramNames, paramTypesMap));
+          var subEnv := env.ToOwned().merge(Environment(paramNames, paramTypesMap, {}));
 
           var recursiveGen, recIdents, _ := GenStmts(body, if selfIdent != NoSelf then ThisTyped("_this", selfIdent.dafnyType) else NoSelf, subEnv, true, None);
           readIdents := {};
@@ -3831,7 +3833,7 @@ module {:extern "DCOMP"} DafnyToRustCompiler {
             readIdents := readIdents + recIdents;
           }
 
-          var newEnv := Environment(paramNames, paramTypes);
+          var newEnv := Environment(paramNames, paramTypes, {});
 
           var recGen, recOwned, recIdents := GenExpr(expr, selfIdent, newEnv, expectedOwnership);
           readIdents := recIdents - paramNamesSet;
